Implementation of rewriting under lambdas. Tested on exists only. Adds some instances that incur again a small performance penalty because they cannot be discriminated against for now (the discrimination net is considering the head constructor to be Morphism).
git-svn-id: svn+ssh://scm.gforge.inria.fr/svn/coq/trunk@10694 85f007b7-540e-0410-9357-904b9bb8a0f7

theories/Classes/RelationClasses.v
@@ -40,6 +40,9 @@ Definition inverse {A} : relation A -> relation A := flip.
 
 Definition complement {A} (R : relation A) : relation A := fun x y => R x y -> False.
 
+Definition pointwise_relation {A B : Type} (R : relation B) : relation (A -> B) := 
+  fun f g => forall x : A, R (f x) (g x).
+
 (** These are convertible. *)
 
 Lemma complement_inverse : forall A (R : relation A), complement (inverse R) = inverse (complement R).
